More wip

CoqOfRust/revm/revm_interpreter/simulations/gas.v
@@ -14,7 +14,18 @@ Module Impl_MemoryGas.
   Definition Self : Set :=
     MemoryGas.t.
 
-  Instance run_new Stack :
+  (* pub const fn new() -> Self *)
+  Instance run_new Stack (stack : Stack.to_Set Stack) :
+    Run.C Impl_MemoryGas.run_new (fun _ => unit) stack.
+  Proof.
+    constructor.
+    apply Run.Pure.
+    exact tt.
+  Defined.
+
+  (* Compute run_new. *)
+
+  (* Instance run_new Stack :
     Run.Trait Stack Impl_MemoryGas.run_new.
   Proof.
     constructor.
@@ -26,7 +37,39 @@ Module Impl_MemoryGas.
     (Output.Success Impl_Default_for_MemoryGas.default, tt).
   Proof.
     reflexivity.
-  Qed.
+  Qed. *)
+
+  (* pub fn record_new_len(&mut self, new_num: usize) -> Option<u64> *)
+  Instance run_record_new_len Stack (stack : Stack.to_Set Stack)
+      (self : Ref.t Pointer.Kind.MutRef Self)
+      (new_num : Usize.t)
+      (H_self : Stack.CanAccess.t Stack self.(Ref.core)) :
+    Run.C (Impl_MemoryGas.run_record_new_len self new_num) (fun _ => unit) stack.
+  Proof.
+    constructor.
+    Ltac simulate_reduce :=
+      repeat match goal with
+      | |- {{ StackM.let_ _ _ 🌲 _ }} =>
+        unfold StackM.let_
+      | |- {{ ?e 🌲 _ }} =>
+        let e' := eval hnf in e in
+        change e with e'
+      end.
+
+    Ltac simulate_get_can_access :=
+      match goal with
+      | |- {{ StackM.GetCanAccess _ _ _ 🌲 _ }} =>
+        unshelve eapply Run.GetCanAccess; [Stack.CanAccess.infer |]
+      end.
+
+    Time simulate_reduce; unshelve eapply Run.GetCanAccess. {
+      Time Stack.CanAccess.infer.
+    }
+    Time try (simulate_reduce; simulate_get_can_access).
+    simulate_reduce.
+    cbn.
+    Show.
+  Defined.
 End Impl_MemoryGas.
 
 Module Impl_Gas.
@@ -34,6 +77,41 @@ Module Impl_Gas.
 
   Definition Self : Set :=
     Gas.t.
+
+  Definition run_limit Stack (stack : Stack.to_Set Stack)
+      (self : Ref.t Pointer.Kind.Ref Self)
+      (H_self : Stack.CanAccess.t Stack self.(Ref.core)) :
+    RunEval.t (Impl_Gas.run_limit self).(Run.run_f) stack.
+  Proof.
+    unfold RunEval.t; cbn.
+    unshelve econstructor. {
+      repeat Stack.CanAccess.infer.
+    }
+    match goal with
+    | |- Run.t (match ?e with _ => _ end) =>
+      destruct e
+    end; constructor.
+  Defined.
+
+  Parameter limit : U64.t.
+
+  Definition self : Ref.t Pointer.Kind.Ref Self := Ref.immediate Pointer.Kind.Ref {|
+    Gas.limit := limit;
+    Gas.remaining := limit;
+    Gas.refunded := {| Integer.value := 0 |};
+    Gas.memory := Impl_Default_for_MemoryGas.default;
+  |}.
+
+  Definition H_self : Stack.CanAccess.t [] self.(Ref.core).
+  Proof.
+    repeat Stack.CanAccess.infer.
+  Defined.
+
+  Compute Run.eval (run_limit [] tt self H_self).
+
+  Compute fun self => Run.eval (
+    run_limit [] tt {| Ref.core := Ref.Core.Immediate (Some self) |} ltac:(now repeat Stack.CanAccess.infer)
+  ).
 
   (*
       pub const fn new(limit: u64) -> Self {
