CoqOfRust/revm/revm_interpreter/instructions/simulations/arithmetic.v
@@ -23,6 +23,7 @@ Proof.
   destruct run_InterpreterTypes_for_WIRE.
   destruct run_StackTrait_for_Stack, run_LoopControl_for_Control.
   simulate_one_step.
+  simulate_one_step.
   simulate.
   { admit. }
   { 
